\section{Ableiten}
\subsection{Ableitungsregeln}
\subsubsection{Faktorregel}
\begin{align*}
    (c \cdot f)(x)' = c \cdot f'(x)
\end{align*}
\subsubsection{Summenregel}
\begin{align*}
    (f+ g)(x)' = f'(x) + g'(x)
\end{align*}
\subsubsection{Produktregel}
\begin{align*}
    (u \cdot v)'(x) = u'(x) \cdot v(x) + u(x) \cdot v'(x)
\end{align*}
\subsubsection{Quotientenregel}
\begin{align*}
    \left(\frac{u}{v}\right)'(x) = \frac{u'(x) \cdot v(x) - u(x) \cdot v'(x)}{(v(x))^2}
\end{align*}
\subsubsection{Kettenregel}
\begin{align*}
    (F \circ u)'(x) = F'(u) \cdot u'(x)
\end{align*}
\subsection{Ableitungen bestimmter Funktionen}
\begin{itemize}
    \item $sin(x)' = cos(x)$
    \item $cos(x)' = -sin(x)$
    \item $(e^x)' = e^x$
    \item $(e^{-20x})' = -3 \cdot e^{-3x}$
    \item $(a^x)' = a^x \cdot ln(a)$
    \item $(ln(x))' = \frac{1}{x}$
    \item $(log_a(x))' = \frac{1}{x \cdot ln(a)}$
\end{itemize}
\subsection{Linearisierung einer Funktion}
Die Funktionsgleichung f√ºr die Tangente von $f(x)$ an der Stelle $x_0$ lautet:
\begin{align*}
    y = f'(x_0) \cdot (x - x_0) + f(x_0)
\end{align*}
\subsection{Newton-Verfahren}
\begin{align*}
    x_{n+1} = x_n - \frac{f(x_n)}{f'(x_n)}
\end{align*}