\section{Folgen und Reihen}
\subsection{Folgen}
\subsubsection{Arithmetische Folge}
\begin{align*}
	a_n & = c + (n-1) \cdot d
\end{align*}
\subsubsection{Geometrische Folge}
\begin{align*}
	a_n & = c \cdot q^{n-1}
\end{align*}
\subsubsection{Grenzwert von Folgen}
%TODO
\subsection{Rechnen mit Grenzwerten}
\begin{align*}
	\lim_{n \to \infty} c \cdot a_n & = c \cdot \lim_{n \to \infty} a_n
\end{align*}
\begin{align*}
	\lim_{n \to \infty} (a_n + b_n) & = \lim_{n \to \infty} a_n + \lim_{n \to \infty} b_n
\end{align*}
\begin{align*}
	\lim_{n \to \infty} (a_n \cdot b_n) & = \lim_{n \to \infty} a_n \cdot \lim_{n \to \infty} b_n
\end{align*}
\begin{align*}
	\lim_{n \to \infty}(\frac{a_n}{b_n}) & = \frac{\lim_{n \to \infty} a_n}{\lim_{n \to \infty} b_n}
\end{align*}
\subsubsection{Arithmetische Reihe}
\begin{align*}
    s_n & =n \cdot a_1 + \frac{n \cdot (n-1)}{2} \cdot d
\end{align*}
\subsubsection{Geometrische Reihe}
\begin{align*}
    s_n & = \frac{a_1 \cdot (1-q^n)}{1-q}
\end{align*}
\subsubsection{Grenzwert von Reihen}
%TODO
